<?xml version="1.0" encoding="iso-8859-1" ?>
<rdf:RDF xmlns:rdf="http://www.w3.org/1999/02/22-rdf-syntax-ns#"
xmlns:rdfs="http://www.w3.org/2000/01/rdf-schema#"
xmlns:owl="http://www.w3.org/2002/07/owl#"
>

<rdf:Property rdf:about="http://fabl.net/vocabularies/geography/map/1.1/boundedBy">
<rdfs:domain rdf:resource="http://www.w3.org/2003/01/geo/wgs84_pos#SpatialThing"/>
<rdfs:range rdf:resource="http://fabl.net/vocabularies/geometry2d/1.1/Shape"/>
</rdf:Property>


<rdf:Property rdf:about="http://fabl.net/vocabularies/geography/map/1.1/envelops">
<owl:inverseOf rdf:resource="http://fabl.net/vocabularies/geography/map/1.1/boundedBy"/>
</rdf:Property>


<owl:FunctionalProperty rdf:about="http://fabl.net/vocabularies/geography/map/1.1/edgeOf">
<rdfs:domain rdf:resource="http://www.w3.org/2003/01/geo/wgs84_pos#SpatialThing"/>
<rdfs:range rdf:resource="http://fabl.net/vocabularies/geometry2d/1.1/Shape"/>
<rdfs:comment>Asserts tthat the edge or boundary of a geo:SpatialThing (such as a park or body of water) is a specified geom2d:Shape.</rdfs:comment>
</owl:FunctionalProperty>


<owl:FunctionalProperty rdf:about="http://fabl.net/vocabularies/geography/map/1.1/isEdgeOf">
<owl:inverseOf rdf:resource="http://fabl.net/vocabularies/geography/map/1.1/edgeOf"/>
</owl:FunctionalProperty>


<owl:FunctionalProperty rdf:about="http://fabl.net/vocabularies/geography/map/1.1/centerLineOf">
<rdfs:domain rdf:resource="http://www.w3.org/2003/01/geo/wgs84_pos#SpatialThing"/>
<rdfs:range rdf:resource="http://fabl.net/vocabularies/geometry2d/1.1/Shape"/>
<rdfs:comment>Asserts that the center line of a linear feature, such as a road or river, is a specified geom2d:Shape.</rdfs:comment>
</owl:FunctionalProperty>


<owl:FunctionalProperty rdf:about="http://fabl.net/vocabularies/geography/map/1.1/isCenterLineOf">
<owl:inverseOf rdf:resource="http://fabl.net/vocabularies/geography/map/1.1/centerLineOf"/>
</owl:FunctionalProperty>


<owl:FunctionalProperty rdf:about="http://fabl.net/vocabularies/geography/map/1.1/srs">
<rdfs:comment>Spatial reference system</rdfs:comment>
</owl:FunctionalProperty>

<rdfs:Class  about="ttp://fabl.net/vocabularies/geography/map/1.1/Map"/>

<owl:FunctionalProperty rdf:about="http://fabl.net/vocabularies/geography/map/1.1/basemap">
<rdfs:domain rdf:resource="http://fabl.net/vocabularies/geography/map/1.1/Map"/>
<rdfs:comment>Background image</rdfs:comment>
</owl:FunctionalProperty>


<owl:FunctionalProperty rdf:about="http://fabl.net/vocabularies/geography/map/1.1/thumbnail">
<rdfs:domain rdf:resource="http://fabl.net/vocabularies/geography/map/1.1/Map"/>
<rdfs:comment>thumbnail specifies a small image used to denote the map in web documents.</rdfs:comment>
</owl:FunctionalProperty>



<owl:FunctionalProperty rdf:about="http://fabl.net/vocabularies/geography/map/1.1/coverage">
<rdfs:domain rdf:resource="http://fabl.net/vocabularies/geography/map/1.1/Map"/>
<rdfs:range rdf:resource="http://fabl.net/vocabularies/geometry2d/1.1/Box"/>
<rdfs:comment>The coverage of a map specifies the range of points on the earth that the map covers, using the map's srs.</rdfs:comment>
</owl:FunctionalProperty>




<owl:FunctionalProperty rdf:about="http://fabl.net/vocabularies/geography/map/1.1/extent">
<rdfs:domain rdf:resource="http://fabl.net/vocabularies/geography/map/1.1/Map"/>
<rdfs:range rdf:resource="http://fabl.net/vocabularies/geometry2d/1.1/Box"/>
<rdfs:comment>The extent is the box representing the map's viewport onto the canvas.</rdfs:comment>
</owl:FunctionalProperty>


<rdf:Property rdf:about="http://fabl.net/vocabularies/geography/map/1.1/canvas">
<rdfs:range rdf:resource="http://fabl.net/vocabularies/geography/map/1.1/Map"/>
<rdfs:comment>This property is an alternative to srs, and is applicable to any located entity (such as a Point or an RSS channel or item, or even another Map).
  If a resource has the canvas property, the values of the x and y properties of its contents are interpreted in the canvas coordinates of the map that is the value of canvas.
</rdfs:comment>
</rdf:Property>


<rdf:Property rdf:about="http://fabl.net/vocabularies/geography/map/1.1/useMap">
<rdfs:range rdf:resource="http://fabl.net/vocabularies/geography/map/1.1/Map"/>
<rdfs:comment>The useMap property asserts that its value is a map that can be used to depict its subject.
For example, an RSS channel might have a useMap property whose value is a map recommended for depicting the contents of the channel.</rdfs:comment>
</rdf:Property>


</rdf:RDF>
